Optimize LV2F by using dlist

experiment/Experiment.Steel.Repr.LV_to_SF.fsti
@@ -15,86 +15,93 @@ open Experiment.Steel.VPropList
 open Experiment.Steel.Repr.LV
 
 #set-options "--fuel 1 --ifuel 1"
+(**) private val __begin_module : unit
 
 irreducible let __LV2SF__ : unit = ()
 
 [@@ __LV2SF__]
-let rec len_eff (#a : Type) (l : list a) : (n : nat { n == L.length l }) =
+let rec len_eff (#a : Type) (l : list a) : n : nat { n == L.length l } =
   match l with
   | [] -> 0
   | _ :: l -> 1 + len_eff l
 
 [@@ __LV2SF__]
-let rec index_eff (#a : Type) (l : list a) (i : Ll.dom l) : (x : a { x == L.index l i }) =
+let rec index_eff (#a : Type) (l : list a) (i : Ll.dom l) : x : a { x == L.index l i } =
   let hd :: tl = l in
   if i = 0 then hd else index_eff tl (i-1)
 
 [@@ __LV2SF__]
-let eij_sl_eff (#src #trg : vprop_list) (eij : eq_injection_l src trg) (xs : sl_f trg)
-  : (sl : sl_f src { sl == eij_sl (L.index eij) xs })
+let dl_initi_vp (v : vprop_list) (f : (i : Ll.dom v) -> Tot (L.index v i).t)
+  : sl_list v
   =
-    let sl = Fl.mk_flist (vprop_list_sels_t src) (fun i -> xs (index_eff eij i) <: (L.index src i).t) in
-    (**) Fl.flist_extensionality sl (eij_sl (L.index eij) xs) (fun i -> ());
+    let n = len_eff v in
+    let f_ty (i : Ll.dom v) : Type = (index_eff v i).t in
+    (**) Ll.list_extensionality (vprop_list_sels_t v) (Ll.initi 0 n f_ty) (fun _ -> ());
+    Dl.initi 0 n f_ty f
+
+
+[@@ __LV2SF__]
+let eij_sl_l (#src #trg : vprop_list) (eij : eq_injection_l src trg) (xs : sl_list trg)
+  : sl : sl_list src { Fl.flist_of_d sl == eij_sl (L.index eij) (Fl.flist_of_d xs) }
+  =
+    let sl = dl_initi_vp src (fun i -> Dl.index xs (index_eff eij i) <: (L.index src i).t) in
+    (**) Fl.flist_extensionality (Fl.flist_of_d sl) (eij_sl (L.index eij) (Fl.flist_of_d xs)) (fun i -> ());
     sl
 
 [@@ __LV2SF__]
-let split_vars_eff (v0 v1 : vprop_list) (sl : sl_f L.(v0 @ v1))
-  : (sls : (sl_f v0 & sl_f v1) { sls == split_vars v0 v1 sl })
+let split_vars_l (v0 v1 : vprop_list) (sl : sl_list L.(v0 @ v1))
+  : sls : (sl_f v0 & sl_f v1) { sls == split_vars v0 v1 (Fl.flist_of_d sl) }
   =
     let n = len_eff v0 in
     (**) Ll.pat_append ();
-    let sl0 = Fl.mk_flist (vprop_list_sels_t v0) (fun i -> sl i       <: (L.index v0 i).t) in
-    let sl1 = Fl.mk_flist (vprop_list_sels_t v1) (fun i -> sl (n + i) <: (L.index v1 i).t) in
-    (**) Fl.flist_extensionality sl0 (split_vars v0 v1 sl)._1 (fun i -> ());
-    (**) Fl.flist_extensionality sl1 (split_vars v0 v1 sl)._2 (fun i -> ());
+    let sl0  = Fl.mk_flist (vprop_list_sels_t v0) (fun i -> Dl.index sl i       <: (L.index v0 i).t) in
+    let sl1  = Fl.mk_flist (vprop_list_sels_t v1) (fun i -> Dl.index sl (n + i) <: (L.index v1 i).t) in
+    let sls' = split_vars v0 v1 (Fl.flist_of_d sl) in
+    (**) Fl.flist_extensionality sl0 sls'._1 (fun i -> ());
+    (**) Fl.flist_extensionality sl1 sls'._2 (fun i -> ());
     (sl0, sl1)
 
 [@@ __LV2SF__]
-let append_vars_eff (#v0 #v1 : vprop_list) (sl0 : sl_f v0) (sl1 : sl_f v1)
-  : (sl : sl_f L.(v0 @ v1) { sl == append_vars sl0 sl1 })
+let append_vars_l (#v0 #v1 : vprop_list) (sl0 : sl_list v0) (sl1 : sl_list v1)
+  : sl : sl_list L.(v0 @ v1) { Fl.flist_of_d sl == append_vars (Fl.flist_of_d sl0) (Fl.flist_of_d sl1) }
   =
-    let n = len_eff v0 in
     (**) Ll.pat_append ();
-    let sl : sl_f L.(v0 @ v1) = Fl.mk_flist L.(vprop_list_sels_t L.(v0 @ v1)) (fun i ->
-      if i < n
-      then (sl0 i <: (L.(index (v0 @ v1) i)).t)
-      else (sl1 (i - n) <: (L.(index (v0 @ v1) i)).t))
-    in
-    (**) Fl.flist_extensionality sl (append_vars sl0 sl1) (fun i -> ());
+    let sl = Dl.append sl0 sl1 in
+    (**) Fl.flist_extensionality (Fl.flist_of_d sl) (append_vars (Fl.flist_of_d sl0) (Fl.flist_of_d sl1))
+    (**)   (fun i -> Dl.append_index sl0 sl1 i);
     sl
 
 [@@ __LV2SF__]
-let res_sel_eff (#env : vprop_list) (sl0 : sl_f env) (csm : csm_t env) (#prd : vprop_list) (sl1 : sl_f prd)
-  : (sl : (sl_f (res_env env csm prd)) { sl == res_sel sl0 csm sl1})
-  = append_vars_eff sl1 (filter_sl (Msk.mask_not csm) sl0)
+let filter_sl_l (#vs : vprop_list) (mask : Msk.mask_t vs) (xs : sl_list vs)
+  : sl : sl_list (Msk.filter_mask mask vs) { Fl.flist_of_d sl == filter_sl mask (Fl.flist_of_d xs) }
+  =
+    (**) Msk.filter_mask_f_dl_f mask _ (Fl.flist_of_d xs);
+    Msk.filter_mask_dl mask _ xs
 
-#push-options "--fuel 0 --ifuel 0"
-(**) private val __begin_opt_0 : unit
 [@@ __LV2SF__]
-let sub_prd_sl_eff
-      (#env : vprop_list) (sl0 : sl_f env)
-      (csm  : csm_t env)  (#prd : vprop_list) (sl1 : sl_f prd)
+let res_sel_l (#env : vprop_list) (sl0 : sl_list env) (csm : csm_t env) (#prd : vprop_list) (sl1 : sl_list prd)
+  : sl : sl_list (res_env env csm prd) { Fl.flist_of_d sl == res_sel (Fl.flist_of_d sl0) csm (Fl.flist_of_d sl1)}
+  =
+    append_vars_l sl1 (filter_sl_l (Msk.mask_not csm) sl0)
+
+[@@ __LV2SF__]
+let extract_vars_l (#src #dst : vprop_list) (p : Perm.pequiv_list src dst) (xs : sl_list src)
+  : ys : sl_list dst { Fl.flist_of_d ys == extract_vars (Perm.perm_f_of_list p) (Fl.flist_of_d xs) }
+  =
+    let ys = dl_initi_vp dst (fun i -> Dl.index xs (index_eff p i)) in
+    (**) Fl.flist_extensionality (Fl.flist_of_d ys) (extract_vars (Perm.perm_f_of_list p) (Fl.flist_of_d xs))
+    (**)   (fun i -> ());
+    ys
+
+[@@ __LV2SF__]
+let sub_prd_sl_l
+      (#env : vprop_list) (sl0 : sl_list env)
+      (csm  : csm_t env)  (#prd : vprop_list) (sl1 : sl_list prd)
       (csm' : csm_t Msk.(filter_mask (mask_not csm) env))
       (#prd' : vprop_list) (prd_f : Perm.pequiv_list (sub_prd env csm prd csm') prd')
-  : (sl : sl_f prd' { sl == sub_prd_sl sl0 csm sl1 csm' prd_f })
+  : (sl : sl_list prd' { Fl.flist_of_d sl == sub_prd_sl (Fl.flist_of_d sl0) csm (Fl.flist_of_d sl1) csm' prd_f })
   =
-    let sl_sprd = append_vars_eff sl1 Msk.(filter_sl csm' (filter_sl (mask_not csm) sl0)) in
-    let sl_prd' = Fl.mk_flist (vprop_list_sels_t prd') (fun i ->
-                        sl_sprd (index_eff prd_f i) <: (L.index prd' i).t)                in
-    (**) Fl.flist_extensionality sl_prd' (sub_prd_sl sl0 csm sl1 csm' prd_f) (fun i -> ());
-    sl_prd'
-#pop-options
-(**) private val __end_opt_0 : unit
-
-[@@ __LV2SF__]
-let dlist_of_sl_eff (#v : vprop_list) (sl : sl_f v)
-  : (sl' : Dl.dlist (vprop_list_sels_t v) { sl' == Fl.dlist_of_f sl })
-  =
-    let f_ty (i : Ll.dom v) : Type = (index_eff v i).t in
-    (**) Ll.list_extensionality (Ll.initi 0 (len_eff v) f_ty) (vprop_list_sels_t v) (fun i -> ());
-    let sl' : Dl.dlist (vprop_list_sels_t v) = Dl.initi 0 (len_eff v) f_ty sl in
-    (**) Dl.dlist_extensionality sl' (Fl.dlist_of_f sl) (fun i -> ());
-    sl'
+    extract_vars_l prd_f (append_vars_l sl1 Msk.(filter_sl_l csm' (filter_sl_l (mask_not csm) sl0)))
 
 
 [@@ __LV2SF__; strict_on_arguments [5]] (* strict on [lc] *)
@@ -102,19 +109,19 @@ let rec repr_SF_of_LV
       (#env : vprop_list) (#a : Type u#a) (#t : M.prog_tree a)
       (#csm : csm_t env) (#prd : prd_t a)
       (lc : lin_cond env t csm prd)
-      (sl0 : sl_f env)
+      (sl0 : sl_list env)
   : Tot (SF.prog_tree a (M.post_sl_t prd)) (decreases lc)
   = match lc with
   | LCspec env #a #sp s sh pre_f ->
-      let sl0s = split_vars_eff s.spc_pre s.spc_ro (eij_sl_eff pre_f sl0) in
+      let sl0s = split_vars_l s.spc_pre s.spc_ro (eij_sl_l pre_f sl0) in
       SF.Tspec a (M.post_sl_t s.spc_post) (s.spc_req sl0s._1 sl0s._2) (fun x sl1 -> s.spc_ens sl0s._1 x sl1 sl0s._2)
   | LCret  env #a #x prd csm_f ->
-      SF.Tret a x (M.post_sl_t prd) (dlist_of_sl_eff (eij_sl_eff csm_f sl0))
+      SF.Tret a x (M.post_sl_t prd) (eij_sl_l csm_f sl0)
   | LCbind env #a #b f_csm f_prd cf g_csm g_prd cg ->
       SF.Tbind a b (M.post_sl_t f_prd) (M.post_sl_t g_prd)
                (repr_SF_of_LV cf sl0)
                (fun (x : a) (sl1 : sl_f (f_prd x)) ->
-                  repr_SF_of_LV (cg x) (res_sel_eff sl0 f_csm sl1))
+                  repr_SF_of_LV (cg x) (res_sel_l sl0 f_csm (Fl.dlist_of_f sl1)))
   | LCbindP env #a #b #wp #g csm prd cg ->
       SF.TbindP a b (M.post_sl_t prd) wp (fun (x : a) -> repr_SF_of_LV (cg x) sl0)
   | LCif    env #a #guard #thn #els csm prd cthn cels ->
@@ -125,8 +132,9 @@ let rec repr_SF_of_LV
       SF.Tbind a a (M.post_sl_t prd0) (M.post_sl_t prd1)
                (repr_SF_of_LV cf sl0)
                (fun (x : a) (sl1 : sl_f (prd0 x)) ->
-                  let sl1' : sl_f (prd1 x) = sub_prd_sl_eff #env sl0 csm0 sl1 csm1 (prd_f x) in
-                  SF.Tret a x (M.post_sl_t prd1) (dlist_of_sl_eff sl1'))
+                  let sl1' : sl_list (prd1 x)
+                           = sub_prd_sl_l #env sl0 csm0 (Fl.dlist_of_f sl1) csm1 (prd_f x) in
+                  SF.Tret a x (M.post_sl_t prd1) sl1')
 
 
 (*** Soundness *)
@@ -135,17 +143,17 @@ let sound_SF_of_LV
       (#env : vprop_list) (#a : Type u#a) (#t : M.prog_tree a)
       (#csm : csm_t env) (#prd : prd_t a)
       (lc : lin_cond env t csm prd)
-      (sl0 : sl_f env)
+      (sl0 : sl_list env)
       (sf : SF.prog_tree a (M.post_sl_t prd))
   : prop
   =
-    (tree_req lc sl0 <==> SF.tree_req sf) /\
+    (tree_req lc (Fl.flist_of_d sl0) <==> SF.tree_req sf) /\
     (forall (res : a) (sl1 : sl_f (prd res)) .
-       tree_ens lc sl0 res sl1 <==> SF.tree_ens sf res sl1)
+       tree_ens lc (Fl.flist_of_d sl0) res sl1 <==> SF.tree_ens sf res sl1)
 
 val repr_SF_of_LV_sound
       (#env : vprop_list) (#a : Type u#a) (#t : M.prog_tree a)
       (#csm : csm_t env) (#prd : prd_t a)
       (lc : lin_cond env t csm prd)
-      (sl0 : sl_f env)
+      (sl0 : sl_list env)
   : Lemma (sound_SF_of_LV lc sl0 (repr_SF_of_LV lc sl0))
